Update proof system and proof to use correct circularity rule

coq/all_shallow/proofsystem.v
@@ -1,69 +1,91 @@
 Section domain.
 Variable cfg : Set.
 
-Definition formula env : Type := cfg -> env -> Prop.
+Definition formula env : Type := env -> cfg -> Prop.
 Definition stateless env : Type := env -> Prop.
 (* Definition rule := { env : Type & formula env & formula env }. *)
 Definition system := forall env,
   formula env -> formula env -> Prop.
 
-Definition cons_system env (phi phi' : formula env) (S : system) : system := fun env0 X X0 =>
-  S env0 X X0 \/
-  {H : env = env0 |
-    (forall gamma rho,
-      phi gamma rho <-> eq_rect_r _ X H gamma rho)
-  /\ (forall gamma rho,
-    phi' gamma rho <-> eq_rect_r _ X0 H gamma rho)}.
+Definition in_opt_system (S : option system) env (phi phi' : formula env) : Prop :=
+  match S with
+    | None => False
+    | Some sys => sys env phi phi'
+  end.
 
+Definition cons_system env (phi phi' : formula env) (S : system) : system :=
+  fun env0 X X0 =>
+    S env0 X X0 \/
+    {H : env = env0 | phi = eq_rect_r _ X H /\ phi' = eq_rect_r _ X0 H}.
+
+Definition cons_opt_system env (phi phi' : formula env) (S : option system) : option system :=
+  Some (cons_system env phi phi' (in_opt_system S)).
+
+Definition system_empty (S : option system) : Prop :=
+  match S with
+    | Some _ => False
+    | None => True
+  end.
+
+Definition union_system (C : option system) (S : system) : system :=
+  match C with
+    | None => S
+    | Some S1 =>
+      fun env0 X X0 => S1 env0 X X0 \/ S env0 X X0
+  end.
+  
 (* accepts a rule if all instances come from the relation *)
 Definition system_of_relation (R : cfg -> cfg -> Prop) : system :=
   fun env phi phi' =>
     forall (rho : env) gamma gamma',
-      phi gamma rho -> phi' gamma' rho -> R gamma gamma'.
+      phi rho gamma -> phi' rho gamma' -> R gamma gamma'.
 
-Inductive IS (S : cfg -> cfg -> Prop) (A : system) : forall (strict : bool) env,
+Section FixTransition.
+Variable (S : cfg -> cfg -> Prop).
+
+Inductive IS (C : option system) (A : system) : forall env,
   formula env -> formula env -> Prop :=
-  | is_refl : forall env phi, IS S A false env phi phi
-  | is_step : forall strict env (phi phi' : formula env),
-                (forall e c, phi c e ->
+  | is_refl : forall env phi, system_empty C -> IS C A env phi phi
+  | is_step : forall env (phi phi' : formula env),
+                (forall e c, phi e c ->
                              (exists c2, S c c2) /\
-                             (forall c2, S c c2 -> phi' c2 e)) ->
-                 IS S A strict env phi phi'
-  | is_axiom : forall strict env phi phi',
-                 A env phi phi' -> IS S A strict env phi phi'
-  | is_subst : forall strict env env' f phi phi',
-       IS S A strict env' phi phi' ->
-       IS S A strict env (fun g e => phi g (f e)) (fun g e => phi' g (f e))
-  | is_trans : forall strict env phi phi' phi'',
-       IS S A strict env phi phi' ->
-       IS S A false env phi' phi'' ->
-       IS S A strict env phi phi''
-  | is_case : forall strict env phi phi1 phi',
-       IS S A strict env phi  phi' ->
-       IS S A strict env phi1 phi' ->
-       IS S A strict env (fun e g => phi e g \/ phi1 e g) phi'
-  | is_lf : forall strict env phi phi' psi,
-       IS S A strict env phi phi' ->
-       IS S A strict env (fun g e => phi g e  /\ psi e)
-                         (fun g e => phi' g e /\ psi e)
-  | is_conseq : forall strict env 
+                             (forall c2, S c c2 -> phi' e c2)) ->
+                 IS C A env phi phi'
+  | is_axiom : forall env phi phi',
+                 A env phi phi' -> IS C A env phi phi'
+  | is_subst : forall env env' f phi phi',
+       IS C A env' phi phi' ->
+       IS C A env (fun e g => phi (f e) g) (fun e g => phi' (f e) g)
+  | is_trans : forall env phi phi' phi'',
+       IS C A env phi phi' ->
+       IS None (union_system C A) env phi' phi'' ->
+       IS C A env phi phi''
+  | is_case : forall env phi phi1 phi',
+       IS C A env phi  phi' ->
+       IS C A env phi1 phi' ->
+       IS C A env (fun e g => phi e g \/ phi1 e g) phi'
+  | is_lf : forall env phi phi' psi,
+       IS C A env phi phi' ->
+       IS C A env (fun e g => phi e g  /\ psi e)
+                  (fun e g => phi' e g /\ psi e)
+  | is_conseq : forall env 
        (phi1 phi1' phi2 phi2' : formula env),
-       (forall g e, phi1 g e -> phi1' g e) ->
-       (forall g e, phi2 g e -> phi2' g e) ->
-       IS S A strict env phi1' phi2 ->
-       IS S A strict env phi1 phi2'
+       (forall e g, phi1 e g -> phi1' e g) ->
+       (forall e g, phi2 e g -> phi2' e g) ->
+       IS C A env phi1' phi2 ->
+       IS C A env phi1 phi2'
 (* use embedding projection pair -
    have env, env' bigger,
    env' phi (fun e' => phi' (project e'))
    env (fun e => exists e', extends e e' /\ phi e') phi'
   *)
-  | is_abstr : forall strict env denx
+  | is_abstr : forall env denx
        (phi : formula (env * denx)) (phi' : formula env),
-       IS S A strict (env * denx) phi (fun g rho_and_x => phi' g (fst rho_and_x)) ->
-       IS S A strict env (fun g rho => exists x, phi g (rho , x)) phi'
-  | is_circ : forall strict env phi phi' phi'',
-       IS S A true env phi phi'' ->
-       IS S (cons_system env phi phi' A) false env phi'' phi' ->
-       IS S A strict env phi phi'.
+       IS C A (env * denx) phi (fun rho_and_x g => phi' (fst rho_and_x) g) ->
+       IS C A env (fun rho g => exists x, phi (rho , x) g) phi'
+  | is_circ : forall env phi phi',
+       IS (cons_opt_system env phi phi' C) A env phi phi' ->
+       IS C A env phi phi'.
+End FixTransition.
 
 End domain.
