coq/all_shallow/soundness.v
@@ -15,7 +15,7 @@ Variable cfg : Set.
 Inductive ts (S : system cfg) : cfg -> cfg -> Prop :=
   | ts_step : forall gamma gamma' env phi phi',
     S env phi phi' ->
-    (exists rho, phi gamma rho /\ phi' gamma' rho) ->
+    (exists rho, phi rho gamma /\ phi' rho gamma') ->
     ts S gamma gamma'.
 
 Section FixBaseSystem.
@@ -24,7 +24,7 @@ Section FixBaseSystem.
 Variable SF : cfg -> cfg -> Prop.
 
 Inductive all_reach (env : Type) (phi : formula cfg env) (rho : env) (gamma : cfg) : bool -> Prop :=
-  | reach_here : phi gamma rho -> all_reach phi rho gamma false
+  | reach_here : phi rho gamma -> all_reach phi rho gamma false
   | reach_later : forall strict,
                     (exists gamma', SF gamma gamma') ->
                   (forall gamma', SF gamma gamma' -> all_reach phi rho gamma' false) ->
@@ -36,7 +36,6 @@ Lemma all_reach_unstrict env phi rho gamma strict :
 Proof.
 inversion 1; eauto using all_reach.
 Qed.
-
 
 Section AllReachAdequacy.
 (* Various proofs to check that all_reach is reasonable *)
@@ -52,7 +51,7 @@ Lemma all_reach_reaches :
   forall env (phi : formula cfg env) (rho : env) (gamma gamma' : cfg)
          (t : trace gamma gamma') strict,
     all_reach phi rho gamma strict ->
-    trace_hits (fun cfg => phi cfg rho) t
+    trace_hits (fun cfg => phi rho cfg) t
                \/ all_reach phi rho gamma' false.
 Proof.
 induction t; intros.    
@@ -69,7 +68,7 @@ Qed.
 Lemma all_reach_path :
   forall env (phi : formula cfg env) (rho : env) (gamma : cfg) strict,
     all_reach phi rho gamma strict ->
-    exists gamma', clos SF strict gamma gamma' /\ phi gamma' rho.
+    exists gamma', clos SF strict gamma gamma' /\ phi rho gamma'.
 induction 1.
 exists gamma. split;[auto using clos_refl|assumption].
 destruct H.
@@ -84,13 +83,82 @@ destruct strict;[|apply clos_unstrict];assumption.
 Qed.
 End AllReachAdequacy.
 
+Definition successors (P : cfg -> Prop) : cfg -> Prop :=
+  fun c => forall c', SF c c' -> P c'.
+
+Lemma under_terminates : forall (P : cfg -> Prop) (c : cfg),
+  terminates c SF ->
+  (forall c', clos SF false c c' -> successors P c' -> P c') ->
+  P c.
+Proof.
+induction 1.
+intros.
+apply H1.
+constructor.
+unfold successors; intros.
+apply H0.
+assumption.
+intros c'0 Hstep.
+apply H1.
+refine (clos_trans _ Hstep).
+apply clos_step. assumption.
+Qed.
+
+Definition always (P : cfg -> Prop) : cfg -> Prop :=
+  fun c => forall c', clos SF false c c' -> P c'.
+
+Lemma always_fwd (P : cfg -> Prop) :
+  forall strict g g',
+    clos SF strict g g' ->
+    always P g -> always P g'.
+Proof.
+unfold always; intros.
+apply H0.
+assert (clos SF false g g') by (destruct strict;auto using clos_unstrict).
+eauto using clos.
+Qed.
+
+Lemma succ_always_strict_fwd (P : cfg -> Prop) :
+  forall g g',
+    clos SF true g g' ->
+    successors (always P) g -> always P g'.
+Proof.
+intros.
+rewrite clos_iff_left in H.
+inversion H; subst.
+auto.
+rewrite <- clos_iff_left in H2.
+specialize (H0 _ H1).
+eauto using always_fwd.
+Qed.
+
 (* at points under gamma, the rule holds semantically *)
 Definition gamma_entails parent strict env
   (phi phi' : formula cfg env) :=
   forall rho gamma,
     clos SF false parent gamma ->
-    phi gamma rho ->
+    phi rho gamma ->
     all_reach phi' rho gamma strict.
+
+Definition gamma_entails_alt strict env (phi phi' : formula cfg env) :=
+  always (fun g => forall rho, phi rho g -> all_reach phi' rho g strict).
+
+Lemma entails : forall p s env (phi phi' : formula cfg env),
+  gamma_entails p s phi phi' <-> gamma_entails_alt s phi phi' p.
+firstorder.  
+Qed.
+
+Definition gamma_succ_entails parent strict env
+  (phi phi' : formula cfg env) :=
+  forall gamma', SF parent gamma' -> gamma_entails gamma' strict phi phi'.
+
+Definition gamma_succ_entails_alt strict env (phi phi' : formula cfg env) :=
+  successors (gamma_entails_alt strict phi phi').
+
+Lemma succ_entails : forall p s env (phi phi' : formula cfg env),
+  gamma_succ_entails p s phi phi' <-> gamma_succ_entails_alt s phi phi' p.
+firstorder.  
+Qed.
 
 Lemma gamma_entails_fwd :
   forall (gamma gamma' : cfg),
@@ -102,9 +170,48 @@ Proof.
   unfold gamma_entails. intros. eauto using clos_trans.
 Qed.
 
+Lemma gamma_succ_entails_strict_fwd :
+  forall (gamma gamma' : cfg),
+    clos SF true gamma gamma' ->
+    forall strict env (phi phi' : formula cfg env),
+      gamma_succ_entails gamma strict phi phi'->
+      gamma_entails gamma' strict phi phi'.
+Proof.
+  intros. rewrite clos_iff_left in H.
+  inversion H;subst.
+  firstorder.
+  specialize (H0 _ H1).
+  rewrite <- clos_iff_left in H2.
+  revert H0.
+  apply gamma_entails_fwd.
+  apply clos_unstrict.
+  assumption.
+Qed.
+
 Definition gamma_entails_system parent strict (S : system cfg) :=
   forall env (phi phi' : formula cfg env), S env phi phi' ->
     gamma_entails parent strict phi phi'.
+
+Definition gamma_entails_system_alt strict (S : system cfg) :=
+  always (fun g => forall env (phi phi' : formula cfg env), S env phi phi' ->
+                   forall rho, phi rho g -> all_reach phi' rho g strict).
+
+Lemma entails_system : forall p s S,
+  gamma_entails_system p s S <-> gamma_entails_system_alt s S p.
+firstorder.
+Qed.
+
+Definition gamma_succ_entails_system parent strict (S : system cfg) :=
+  forall gamma', SF parent gamma' -> gamma_entails_system gamma' strict S.
+
+Definition gamma_succ_entails_system_alt strict (S : system cfg) :=
+  successors (gamma_entails_system_alt strict S).
+
+Lemma succ_entails_system : forall p s S,
+  gamma_succ_entails_system p s S <-> gamma_succ_entails_system_alt s S p.
+unfold gamma_succ_entails_system, gamma_succ_entails_system_alt, successors.
+intuition;apply entails_system; auto.
+Qed.
 
 Lemma gamma_system_fwd : forall gamma gamma' strict S,
   clos SF false gamma gamma' ->
@@ -116,14 +223,29 @@ Proof.
   eauto using gamma_entails_fwd.
 Qed.
 
-Lemma all_reach_impl :
-  forall env (phi phi' : formula cfg env) rho gamma strict,
-    (forall gamma rho, phi gamma rho -> phi' gamma rho) ->
+Lemma clos_ext : forall a b c strict,
+                   SF a b -> clos SF strict b c -> clos SF strict b c.
+eauto using clos,clos_unstrict.
+Qed.
+
+Lemma all_reach_impl_path :
+  forall env (phi : formula cfg env) rho env' (phi' : formula cfg env') rho' gamma strict,
+    (forall gamma', clos SF false gamma gamma' ->  phi rho gamma' -> phi' rho' gamma') ->
     all_reach phi rho gamma strict ->
-    all_reach phi' rho gamma strict.
+    all_reach phi' rho' gamma strict.
 Proof.
-intros.
-induction H0; eauto using all_reach.
+intros. induction H0.
+eauto using all_reach, clos.
+apply reach_later;eauto using all_reach, clos, clos_ext.
+Qed.
+
+Lemma all_reach_impl :
+  forall env (phi : formula cfg env) rho env' (phi' : formula cfg env') rho' gamma strict,
+    (forall gamma, phi rho gamma -> phi' rho' gamma) ->
+    all_reach phi rho gamma strict ->
+    all_reach phi' rho' gamma strict.
+Proof.
+intros. induction H0; auto using all_reach.
 Qed.
 
 Lemma gamma_system_cons : forall gamma S env
@@ -146,7 +268,7 @@ Proof.
   specialize (H0 rho gamma0 H H1).
   clear -Hphi' H0.
   revert H0; apply all_reach_impl.
-  apply Hphi'.
+  subst. trivial.
 Qed.
 
 Lemma gamma_entails_unstrict :
@@ -189,6 +311,35 @@ apply gamma_entails_fwd.
 auto using clos_step.
 Qed.
 
+Require Import Bool.
+
+Lemma all_reach_join : forall env (phi : formula cfg env) rho g strict1 strict2,
+  all_reach (fun rho g => all_reach phi rho g strict1) rho g strict2 ->
+  all_reach phi rho g (orb strict1 strict2).
+intros.
+induction H;rewrite orb_false_r in * |- *.
+assumption.
+apply reach_later.
+assumption.
+intros.
+specialize (H0 _ H2).
+specialize (H1 _ H2).
+destruct strict1;[apply all_reach_unstrict|];assumption.
+Qed.
+
+Lemma gamma_entails_trans_nonstrict :
+  forall gamma env (phi phi' phi'' : formula cfg env),
+    gamma_entails gamma false phi phi' ->
+    gamma_entails gamma false phi' phi'' ->
+    gamma_entails gamma false phi phi''.
+Proof.
+  unfold gamma_entails; intros.
+  specialize (H _ _ H1 H2).
+  apply (@all_reach_join _ _ _ _ false false).
+  revert H.
+  apply all_reach_impl_path; eauto using clos_trans.
+Qed.
+
 Lemma gamma_entails_trans :
   forall gamma env (phi phi' phi'' : formula cfg env),
     gamma_entails gamma true phi phi' ->
@@ -222,123 +373,121 @@ Proof.
   auto using clos_refl.
 Qed.
 
-Theorem soundness : forall strict S env phi phi',
-  forall (proof : IS cfg SF S strict env phi phi'),
+Theorem soundness : forall C S env phi phi',
+  forall (proof : IS cfg SF C S env phi phi'),
     forall gamma,
       terminates gamma SF ->
       gamma_entails_system gamma true S ->
-      gamma_entails gamma strict phi phi'.
-
+      match C with
+          | None => True
+          | Some c => gamma_succ_entails_system gamma true c
+      end ->
+      gamma_entails gamma (match C with None => false | Some _ => true end) phi phi'.
 Proof.
   intros until phi'; intro proof.
-  induction proof; intros gamma Hterm Hsystem.
+  induction proof; intros gamma Hterm Hsystem HCsystem.
 
 (* refl *)
-  intro gamma0; intros.
-  solve [firstorder using clos_refl, all_reach].
++ destruct C;[destruct H|].
+  unfold gamma_entails; auto using all_reach.
 
 (* step *)
-  intro;intros.
-  specialize (H rho gamma0 H1).
-  destruct H.
-  apply all_reach_unstrict.
-  constructor.
++ unfold gamma_entails; intros.
+  destruct (H _ _ H1).
+  apply reach_later.
   assumption.
-  intros.
-  specialize (H2 gamma' H3).
-  constructor.
-  assumption.
+  auto using all_reach.
 
 (* axiom *)
-  apply gamma_entails_unstrict.
-  apply gamma_entails_unstrict; solve[auto].
++ apply gamma_entails_unstrict. auto.
 
 (* subst *)
-  specialize (IHproof gamma Hterm Hsystem); clear -IHproof.
-  unfold gamma_entails in * |- *. firstorder.
++ specialize (IHproof gamma Hterm Hsystem HCsystem); clear -IHproof.
+  unfold gamma_entails in * |- *; intros.
   specialize (IHproof (f rho) gamma0 H H0).
-  revert IHproof. clear.
-  solve[induction 1;constructor;(assumption || firstorder)].
+  revert IHproof.
+  apply all_reach_impl.
+  trivial.
 
 (* trans *) 
-  specialize (IHproof1 gamma Hterm Hsystem);
-  specialize (IHproof2 gamma Hterm Hsystem);
++ destruct C.
+  (* true case where we need to take steps *)
+  apply gamma_entails_trans with phi'.
+  apply IHproof1; assumption.
+  intros.
+  apply IHproof2.
+  eauto using terminates_fwd.
+  simpl.
+  assert (gamma_entails_system gamma' true A) by (eauto using clos_unstrict, gamma_system_fwd).
+  assert (gamma_entails_system gamma' true s).
+    rewrite entails_system.
+    rewrite succ_entails_system in HCsystem.
+    eapply succ_always_strict_fwd;eassumption.
+  clear -H0 H1.
+  unfold gamma_entails_system in H0, H1 |- *.
+  intros.
+  firstorder.
+  trivial.
+  (* false case, where we don't need to prove anything about C *)
+  specialize (IHproof1 _ Hterm Hsystem I).
+  specialize (IHproof2 _ Hterm Hsystem I).
   clear -IHproof1 IHproof2.
-  unfold gamma_entails.
-  intros.
-  specialize (IHproof1 rho gamma0 H H0).
-  destruct IHproof1.
-  apply IHproof2; assumption.
-  (* if it took a step, stuff *)
-  constructor.
-  assumption.
-  intros.
-  specialize (H2 gamma' H3).
-  assert (clos SF false gamma gamma') by (eauto using clos).
-  apply (gamma_entails_fwd H4) in IHproof2.
-  revert IHproof2 H2; clear.
-  solve[apply all_step_trans].
+  eapply gamma_entails_trans_nonstrict;eassumption.
 
 (* ps_case *)
-  solve[firstorder].
++ solve[firstorder].
 
 (* ps_lf *)
-  specialize (IHproof gamma Hterm Hsystem).
++ specialize (IHproof gamma Hterm Hsystem HCsystem).
   revert IHproof; clear.
   intro; intro; intros.
   destruct H0.
   specialize (IHproof rho gamma0 H H0).
   clear -IHproof H1.
-  induction IHproof;constructor;solve[auto].
+  revert IHproof; apply all_reach_impl. auto.
 
 (* ps_conseq *)
-  specialize (IHproof gamma Hterm Hsystem).
++ specialize (IHproof gamma Hterm Hsystem HCsystem).
   intros rho gamma0; intros.
   apply H in H2.
   specialize (IHproof rho gamma0 H1 H2).
   revert IHproof.
   apply all_reach_impl.
-  assumption.
+  auto.
 
 (* ps_abstr *)
-  specialize (IHproof gamma Hterm Hsystem).
++ specialize (IHproof gamma Hterm Hsystem HCsystem).
   intro; intros.
   destruct H0.
   specialize (IHproof (rho , x) gamma0 H H0).
-  clear -IHproof.
-  induction IHproof;constructor;assumption.
+  revert IHproof. apply all_reach_impl. auto.
 
 (* ps_circ *)
-  specialize (IHproof1 gamma Hterm Hsystem).
-
-  assert (forall gamma2,
-    clos SF true gamma gamma2 ->
-    gamma_entails gamma2 true phi phi' ->
-    gamma_entails gamma2 false phi'' phi').
++ apply gamma_entails_unstrict.
+  pattern gamma.
+  apply under_terminates.
+  assumption.
   intros.
-  apply IHproof2;[solve[eauto using terminates_fwd]|].
-  apply gamma_system_cons;[|assumption].
-  clear -Hsystem H.
-  unfold gamma_entails_system.
-  intros. specialize (Hsystem env phi phi' H0).
-  eauto using gamma_entails_fwd, clos_unstrict.
-
-  clear IHproof2.
-  rename H into IHproof2.
-
-  cut (gamma_entails gamma true phi phi').
-  apply gamma_entails_unstrict.
-
-  apply terminates_trans in Hterm.
-  revert Hterm. induction 1.
-
-  eapply gamma_entails_trans;[eassumption|].
+  apply IHproof.
+  eauto using terminates_fwd.
+  eauto using gamma_system_fwd.
+  simpl.
+  unfold gamma_succ_entails_system, gamma_entails_system.
   intros.
-  apply IHproof2;[assumption|].
-
-  apply H0;
-    eauto using gamma_entails_fwd, gamma_system_fwd,
-      clos_unstrict, clos_trans.
+  destruct H2.
+  destruct C;[|destruct H2].
+  simpl in H2.
+  assert (clos SF true gamma gamma').
+  eapply clos_cons_rt. eassumption. constructor (assumption).
+  apply gamma_succ_entails_strict_fwd with gamma.
+  assumption.
+  clear -H2 HCsystem.
+  unfold gamma_succ_entails. intros.
+  specialize (HCsystem _ H _ _ _ H2). assumption.
+  destruct H2 as [<- []].
+  unfold eq_rect_r, eq_sym in H2, H3; simpl in H2, H3; subst phi0 phi'0.
+  specialize (H0 _ H1); simpl in H0.
+  assumption.
 Qed.
 
 Definition empty_system : system cfg := fun env phi phi' => False.
@@ -348,12 +497,12 @@ unfold gamma_entails_system; simpl; intros.
 destruct H.
 Qed.
 
-Theorem simple_soundness : forall strict env phi phi',
-  IS cfg SF empty_system strict env phi phi' ->
+Theorem simple_soundness : forall env phi phi',
+  IS cfg SF None empty_system env phi phi' ->
   forall gamma : cfg, terminates gamma SF ->
-  forall rho, phi gamma rho -> all_reach phi' rho gamma strict.
+  forall rho, phi rho gamma -> all_reach phi' rho gamma false.
 intros.
-eapply soundness; eauto using empty_system_vacuous, clos_refl.
+eapply soundness with (C:= None); eauto using empty_system_vacuous, clos_refl.
 Qed.
 
 End FixBaseSystem.
